src/hog/HoG.lean
@@ -1,8 +1,7 @@
-import TreeSet
-import TreeMap
-import Graph
 import GraphJson
-import Tactic
-import ConnectedComponents
-import Walk
-import Query
+
+namespace HoG
+
+
+
+end HoG
