src/hog/JsonDecoder.lean
@@ -1,0 +1,52 @@
+import Qq
+import Graph
+
+set_option autoImplicit false
+
+namespace HoG
+
+open Qq
+
+def edgeOfJson (n : Q(Nat)) (j : Lean.Json) : Except String Q(Edge $n) := do
+  let arr ← j.getArr?
+  have a : Q(Nat) := Lean.mkRawNatLit (← arr[0]!.getNat?)
+  have b : Q(Nat) := Lean.mkRawNatLit (← arr[1]!.getNat?)
+  have H1 : Q(Nat.blt $a $n = true) := (q(Eq.refl true) : Lean.Expr)
+  have H2 : Q(Nat.blt $b $a = true) := (q(Eq.refl true) : Lean.Expr)
+  pure q(Edge.mk' $n $a $b $H1 $H2)
+
+partial def treeOfJson (n : Q(Nat)) (j : Lean.Json) : Except String Q(STree (Edge $n)) := do
+  let arr ← j.getArr? 
+  match arr with
+  | #[e, l, r] => pure q(STree.node $(← edgeOfJson n e) $(← treeOfJson n l) $(← treeOfJson n r))
+  | #[] => pure q(STree.empty)
+  | #[v] => pure q(STree.leaf $(← edgeOfJson n v))
+  | _ => throw "invalid tree format"
+
+partial def graphOfJson (j : Lean.Json) : Except String Q(Graph) := do
+    let njson ← j.getObjVal? "vertexSize"
+    have n : Q(Nat) := Lean.mkRawNatLit (← njson.getNat?)
+    let edges : Q(STree (Edge $n)) ← (treeOfJson n (← j.getObjVal? "edges"))
+    pure q(Graph.mk $n $edges) -- here it dies with: reduceEval: failed to evaluate argument __do_lift✝¹
+
+elab "getHog" hogId:str : command => do
+  let packageDir ← Mathlib.getPackageDir "HoG"
+  let dataDir := ((packageDir.join "..").join "..").join "pigpen" -- folder with the JSON files
+  let fileName := (dataDir.join hogId.getString).withExtension "json"
+  let file ← IO.FS.readFile fileName
+  let graph : Except String (Q(Graph)) := do
+    let json ← Lean.Json.parse file 
+    graphOfJson json
+  let .ok value := graph | throwError "could not load the JSON file"
+  Lean.Elab.Command.liftCoreM <| Lean.addDecl <| .defnDecl {
+    name := (.str (.str .anonymous "HoG") hogId.getString)
+    levelParams := []
+    type := q(Graph)
+    value
+    hints := .regular 0
+    safety := .safe
+  }
+  
+-- getHog "hog00000"
+
+end HoG
